WIP: Finally a promising approach via `insertLast''`

RuleSystem/Rules/Wip.lean
@@ -1,9 +1,45 @@
 import RuleSystem.Rules.Theorems.Advanced
 
+namespace Instance
+
+def insertLast {n : ℕ} (inst : Instance (n + 1)) : Instance (n + 1)
+  := ⟨inst.tags ∪ {Fin.last _}⟩
+
+def insertLast'' {n : ℕ} (rule : Rule n) (inst : rule.captureEmbed) : Instance (n + 1)
+  := ⟨inst.val.tags ∪ {Fin.last _}⟩
+
+theorem insertLast''_injective {n : ℕ} (rule : Rule n) : Function.Injective (insertLast'' rule) := by
+  sorry
+
+def insertLast''Embedding {n : ℕ} (rule : Rule n) : rule.captureEmbed ↪ Instance (n + 1)
+  := ⟨insertLast'' rule, insertLast''_injective rule⟩
+
+-- -- def Finset.restrict {ι : Type u_2} {π : ι → Type u_3} (s : Finset ι) (f : (i : ι) → π i) (i : { x : ι // x ∈ s }) :
+-- -- π ↑i
+-- --
+-- -- ι =
+-- def restrictInsertLast {n : ℕ} (inst : Instance (n + 1)) (h : inst.CastPredPrecondition) : Instance (n + 1)
+--   := Finset.restrict (Instances.notContainingLast n) insertLast _
+
+end Instance
+
 namespace Rule
+
+-- TODO: Fix this
+def captureEmbedInsertLast {n : ℕ} (rule : Rule n) : Instances (n + 1)
+  := rule.captureEmbed.map (Instance.insertLast''Embedding rule)
+
+-- def captureEmbedEmbedding
+
+-- instance {n : ℕ} (rule : Rule n) : CoeDep (Instances (n + 1)) rule.captureEmbed (Finset (@Instances.notContainingLast n)) where
+--   coe := by
+--     exists rule.captureEmbed.map (Subtype (· ∈ @Instances.notContainingLast n))
+
+--     sorry
 
 
 -- TODO: Finish this 🍊
+-- (Instances.insertLast' rule.val.captureEmbed)
 -- application type mismatch
 --   Instances.insertLast' (↑rule).captureEmbed
 -- argument
@@ -14,9 +50,11 @@ namespace Rule
 --   Finset { x // x ∈ Instances.notContainingLast } : Type
 
 -- This is probably wrong / not what we want
--- instance CoeDepCaptureEmbedNotContainingLast {n : ℕ} (rule : Rule n)
---   : CoeDep (Instances (n + 1)) rule.captureEmbed (Finset (@Instances.notContainingLast n)) where
+-- instance CoeDepCaptureEmbedNotContainingLast {n : ℕ} (rule : Rule n) (x : Instances (n + 1)) (h : x = rule.captureEmbed)
+--   : CoeDep (Instances (n + 1)) x (Finset (@Instances.notContainingLast n)) where
 --     coe := by
+--       exists x.val
+
 --       -- exists rule.captureEmbed
 --       sorry
 
